create module, indent the things, also rewrite [nils] to use tuple [repeat] and prove [nils] correct

src/SaturatedBaseSystem.v
@@ -16,167 +16,198 @@ saturated limbs. Compatible with mixed-radix bases.
 
  ***)
 
-Section Saturated.
-  Context {weight : nat->Z}
-          {weight_0 : weight 0%nat = 1}
-          {weight_nonzero : forall i, weight i <> 0}
-          {weight_multiples : forall i, weight (S i) mod weight i = 0}
-          (* add_get_carry takes in a number at which to split output *)
-          {add_get_carry: Z ->Z -> Z -> (Z * Z)}
-          {add_get_carry_correct : forall s x y,
-              fst (add_get_carry s x y)  = x + y - s * snd (add_get_carry s x y)}
-  .
+Module Sorted.
+  Section Saturated.
+    Context {weight : nat->Z}
+            {weight_0 : weight 0%nat = 1}
+            {weight_nonzero : forall i, weight i <> 0}
+            {weight_multiples : forall i, weight (S i) mod weight i = 0}
+            (* add_get_carry takes in a number at which to split output *)
+            {add_get_carry: Z ->Z -> Z -> (Z * Z)}
+            {add_get_carry_correct : forall s x y,
+                fst (add_get_carry s x y)  = x + y - s * snd (add_get_carry s x y)}
+    .
 
-  Definition eval {n} (x : (list Z)^n) : Z :=
-    B.Positional.eval weight (Tuple.map sum x).
+    Definition eval {n} (x : (list Z)^n) : Z :=
+      B.Positional.eval weight (Tuple.map sum x).
 
-  Definition eval_from {n} (offset:nat) (x : (list Z)^n) : Z :=
-    B.Positional.eval (fun i => weight (i+offset)) (Tuple.map sum x).
+    Definition eval_from {n} (offset:nat) (x : (list Z)^n) : Z :=
+      B.Positional.eval (fun i => weight (i+offset)) (Tuple.map sum x).
 
-  Lemma eval_from_0 {n} x : @eval_from n 0 x = eval x.
-  Proof. cbv [eval_from eval]. auto using B.Positional.eval_wt_equiv. Qed.
+    Lemma eval_from_0 {n} x : @eval_from n 0 x = eval x.
+    Proof. cbv [eval_from eval]. auto using B.Positional.eval_wt_equiv. Qed.
 
-  Lemma eval_from_S {n}: forall i (inp : (list Z)^(S n)),
-    eval_from i inp = eval_from (S i) (tl inp) + weight i * sum (hd inp).
-  Proof.
-    intros; cbv [eval_from].
-    replace inp with (append (hd inp) (tl inp))
-      by (simpl in *; destruct n; destruct inp; reflexivity).
-    rewrite map_append, B.Positional.eval_step, hd_append, tl_append.
-    autorewrite with natsimplify; ring_simplify; rewrite Group.cancel_left.
-    apply B.Positional.eval_wt_equiv; intros; f_equal; omega.
-  Qed.
+    Lemma eval_from_S {n}: forall i (inp : (list Z)^(S n)),
+        eval_from i inp = eval_from (S i) (tl inp) + weight i * sum (hd inp).
+    Proof.
+      intros; cbv [eval_from].
+      replace inp with (append (hd inp) (tl inp))
+        by (simpl in *; destruct n; destruct inp; reflexivity).
+      rewrite map_append, B.Positional.eval_step, hd_append, tl_append.
+      autorewrite with natsimplify; ring_simplify; rewrite Group.cancel_left.
+      apply B.Positional.eval_wt_equiv; intros; f_equal; omega.
+    Qed.
 
-  (* Sums a list of integers using carry bits.
+    (* Sums a list of integers using carry bits.
      Output : next index, carry, sum
-   *)
-  Fixpoint compact_digit_cps n (digit : list Z) {T} (f:Z * Z->T) :=
-  match digit with
-  | nil => f (0, 0)
-  | x :: nil => f (0, x)
-  | x :: tl =>
-    compact_digit_cps n tl (fun rec =>
-      dlet sum_carry := add_get_carry (weight (S n) / weight n) x (snd rec) in
-      dlet carry' := (fst rec + snd sum_carry)%RT in
-    f (carry', fst sum_carry))
-  end.
+     *)
+    Fixpoint compact_digit_cps n (digit : list Z) {T} (f:Z * Z->T) :=
+      match digit with
+      | nil => f (0, 0)
+      | x :: nil => f (0, x)
+      | x :: tl =>
+        compact_digit_cps n tl (fun rec =>
+                                  dlet sum_carry := add_get_carry (weight (S n) / weight n) x (snd rec) in
+                                    dlet carry' := (fst rec + snd sum_carry)%RT in
+                                    f (carry', fst sum_carry))
+      end.
 
-  Definition compact_digit n digit := compact_digit_cps n digit id.
-  Lemma compact_digit_id n digit: forall {T} f,
-      @compact_digit_cps n digit T f = f (compact_digit n digit).
-  Proof.
-    induction digit; intros; cbv [compact_digit]; [reflexivity|];
-      simpl compact_digit_cps; break_match; [reflexivity|].
-    rewrite !IHdigit; reflexivity.
-  Qed.
-  Hint Opaque compact_digit : uncps.
-  Hint Rewrite compact_digit_id : uncps.
+    Definition compact_digit n digit := compact_digit_cps n digit id.
+    Lemma compact_digit_id n digit: forall {T} f,
+        @compact_digit_cps n digit T f = f (compact_digit n digit).
+    Proof.
+      induction digit; intros; cbv [compact_digit]; [reflexivity|];
+        simpl compact_digit_cps; break_match; [reflexivity|].
+      rewrite !IHdigit; reflexivity.
+    Qed.
+    Hint Opaque compact_digit : uncps.
+    Hint Rewrite compact_digit_id : uncps.
 
-  Definition compact_step_cps (index:nat) (carry:Z) (digit: list Z)
-    {T} (f:Z * Z->T) :=
-    compact_digit_cps index (carry::digit) f.
+    Definition compact_step_cps (index:nat) (carry:Z) (digit: list Z)
+               {T} (f:Z * Z->T) :=
+      compact_digit_cps index (carry::digit) f.
 
-  Definition compact_step i c d := compact_step_cps i c d id.
-  Lemma compact_step_id i c d T f :
-    @compact_step_cps i c d T f = f (compact_step i c d).
-  Proof. cbv [compact_step_cps compact_step]; autorewrite with uncps; reflexivity. Qed.
-  Hint Opaque compact_step : uncps.
-  Hint Rewrite compact_step_id : uncps.
-  
-  Definition compact_cps {n} (xs : (list Z)^n) {T} (f:Z * Z^n->T) := 
-    mapi_with_cps compact_step_cps 0 xs f.
+    Definition compact_step i c d := compact_step_cps i c d id.
+    Lemma compact_step_id i c d T f :
+      @compact_step_cps i c d T f = f (compact_step i c d).
+    Proof. cbv [compact_step_cps compact_step]; autorewrite with uncps; reflexivity. Qed.
+    Hint Opaque compact_step : uncps.
+    Hint Rewrite compact_step_id : uncps.
+    
+    Definition compact_cps {n} (xs : (list Z)^n) {T} (f:Z * Z^n->T) := 
+      mapi_with_cps compact_step_cps 0 xs f.
 
-  Definition compact {n} xs := @compact_cps n xs _ id.
-  Lemma compact_id {n} xs {T} f : @compact_cps n xs T f = f (compact xs).
-  Proof. cbv [compact_cps compact]; autorewrite with uncps; reflexivity. Qed.
+    Definition compact {n} xs := @compact_cps n xs _ id.
+    Lemma compact_id {n} xs {T} f : @compact_cps n xs T f = f (compact xs).
+    Proof. cbv [compact_cps compact]; autorewrite with uncps; reflexivity. Qed.
 
-  Lemma compact_digit_correct i (xs : list Z) :
-    snd (compact_digit i xs)  = sum xs - (weight (S i) / weight i) * (fst (compact_digit i xs)).
-  Proof.
-    induction xs; cbv [compact_digit]; simpl compact_digit_cps;
-      cbv [Let_In];
+    Lemma compact_digit_correct i (xs : list Z) :
+      snd (compact_digit i xs)  = sum xs - (weight (S i) / weight i) * (fst (compact_digit i xs)).
+    Proof.
+      induction xs; cbv [compact_digit]; simpl compact_digit_cps;
+        cbv [Let_In];
+        repeat match goal with
+               | _ => rewrite add_get_carry_correct
+               | _ => progress (rewrite ?sum_cons, ?sum_nil in * )
+               | _ => progress (autorewrite with uncps push_id in * )
+               | _ => progress (autorewrite with cancel_pair in * )
+               | _ => progress break_match; try discriminate
+               | _ => progress ring_simplify
+               | _ => reflexivity
+               | _ => nsatz
+               end.
+    Qed.
+
+    Definition compact_invariant n i (starter rem:Z) (inp : tuple (list Z) n) (out : tuple Z n) :=
+      B.Positional.eval_from weight i out + weight (i + n) * (rem)
+      = eval_from i inp + weight i*starter.
+
+    Lemma compact_invariant_holds n i starter rem inp out :
+      compact_invariant n (S i) (fst (compact_step_cps i starter (hd inp) id)) rem (tl inp) out ->
+      compact_invariant (S n) i starter rem inp (append (snd (compact_step_cps i starter (hd inp) id)) out).
+    Proof.
+      cbv [compact_invariant B.Positional.eval_from]; intros.
       repeat match goal with
-             | _ => rewrite add_get_carry_correct
-             | _ => progress (rewrite ?sum_cons, ?sum_nil in * )
-             | _ => progress (autorewrite with uncps push_id in * )
-             | _ => progress (autorewrite with cancel_pair in * )
-             | _ => progress break_match; try discriminate
+             | _ => rewrite B.Positional.eval_step
+             | _ => rewrite eval_from_S
+             | _ => rewrite sum_cons 
+             | _ => rewrite weight_multiples
+             | _ => rewrite Nat.add_succ_l in *
+             | _ => rewrite Nat.add_succ_r in *
+             | _ => (rewrite fst_fst_compact_step in * )
              | _ => progress ring_simplify
-             | _ => reflexivity
-             | _ => nsatz
+             | _ => rewrite ZUtil.Z.mul_div_eq_full by apply weight_nonzero
+             | _ => cbv [compact_step_cps] in *;
+                      autorewrite with uncps push_id;
+                      rewrite compact_digit_correct
+             | _ => progress (autorewrite with natsimplify in * )
              end.
-  Qed.
+      rewrite B.Positional.eval_wt_equiv with (wtb := fun i0 => weight (i0 + S i)) by (intros; f_equal; try omega).
+      nsatz.
+    Qed.
 
-  Definition compact_invariant n i (starter rem:Z) (inp : tuple (list Z) n) (out : tuple Z n) :=
-    B.Positional.eval_from weight i out + weight (i + n) * (rem)
-    = eval_from i inp + weight i*starter.
+    Lemma compact_invariant_base i rem : compact_invariant 0 i rem rem tt tt.
+    Proof. cbv [compact_invariant]. simpl. repeat (f_equal; try omega). Qed.
 
-  Lemma compact_invariant_holds n i starter rem inp out :
-    compact_invariant n (S i) (fst (compact_step_cps i starter (hd inp) id)) rem (tl inp) out ->
-    compact_invariant (S n) i starter rem inp (append (snd (compact_step_cps i starter (hd inp) id)) out).
-  Proof.
-    cbv [compact_invariant B.Positional.eval_from]; intros.
-    repeat match goal with
-           | _ => rewrite B.Positional.eval_step
-           | _ => rewrite eval_from_S
-           | _ => rewrite sum_cons 
-           | _ => rewrite weight_multiples
-           | _ => rewrite Nat.add_succ_l in *
-           | _ => rewrite Nat.add_succ_r in *
-           | _ => (rewrite fst_fst_compact_step in * )
-           | _ => progress ring_simplify
-           | _ => rewrite ZUtil.Z.mul_div_eq_full by apply weight_nonzero
-           | _ => cbv [compact_step_cps] in *;
-                    autorewrite with uncps push_id;
-                    rewrite compact_digit_correct
-           | _ => progress (autorewrite with natsimplify in * )
-           end.
-    rewrite B.Positional.eval_wt_equiv with (wtb := fun i0 => weight (i0 + S i)) by (intros; f_equal; try omega).
-    nsatz.
-  Qed.
+    Lemma compact_invariant_end {n} start (input : (list Z)^n):
+      compact_invariant n 0%nat start (fst (mapi_with_cps compact_step_cps start input id)) input (snd (mapi_with_cps compact_step_cps start input id)).
+    Proof.
+      autorewrite with uncps push_id.
+      apply (mapi_with_invariant _ compact_invariant
+                                 compact_invariant_holds compact_invariant_base).
+    Qed.
 
-  Lemma compact_invariant_base i rem : compact_invariant 0 i rem rem tt tt.
-  Proof. cbv [compact_invariant]. simpl. repeat (f_equal; try omega). Qed.
+    Lemma eval_compact {n} (xs : tuple (list Z) n) :
+      B.Positional.eval weight (snd (compact xs)) + (weight n * fst (compact xs)) = eval xs.
+    Proof.
+      pose proof (compact_invariant_end 0 xs) as Hinv.
+      cbv [compact_invariant] in Hinv.
+      simpl in Hinv. autorewrite with zsimplify natsimplify in Hinv.
+      rewrite eval_from_0, B.Positional.eval_from_0 in Hinv; apply Hinv.
+    Qed.
 
-  Lemma compact_invariant_end {n} start (input : (list Z)^n):
-    compact_invariant n 0%nat start (fst (mapi_with_cps compact_step_cps start input id)) input (snd (mapi_with_cps compact_step_cps start input id)).
-  Proof.
-    autorewrite with uncps push_id.
-    apply (mapi_with_invariant _ compact_invariant
-                               compact_invariant_holds compact_invariant_base).
-  Qed.
+    Definition cons_to_nth_cps {n} i (x:Z) (t:(list Z)^n)
+               {T} (f:(list Z)^n->T) :=
+      @on_tuple_cps _ _ nil (update_nth_cps i (cons x)) n n t _ f.
 
-  Lemma eval_compact {n} (xs : tuple (list Z) n) :
-    B.Positional.eval weight (snd (compact xs)) + (weight n * fst (compact xs)) = eval xs.
-  Proof.
-    pose proof (compact_invariant_end 0 xs) as Hinv.
-    cbv [compact_invariant] in Hinv.
-    simpl in Hinv. autorewrite with zsimplify natsimplify in Hinv.
-    rewrite eval_from_0, B.Positional.eval_from_0 in Hinv; apply Hinv.
-  Qed.
+    Definition cons_to_nth {n} i x t := @cons_to_nth_cps n i x t _ id.
+    Lemma cons_to_nth_id {n} i x t T f :
+      @cons_to_nth_cps n i x t T f = f (cons_to_nth i x t).
+    Proof.
+      cbv [cons_to_nth_cps cons_to_nth].
+      assert (forall xs : list (list Z), length xs = n ->
+                 length (update_nth_cps i (cons x) xs id) = n) as Hlen.
+      { intros. autorewrite with uncps push_id distr_length. assumption. }
+      rewrite !on_tuple_cps_correct with (H:=Hlen)
+        by (intros; autorewrite with uncps push_id; reflexivity). reflexivity.
+    Qed.
+    Hint Opaque cons_to_nth : uncps.
+    Hint Rewrite @cons_to_nth_id : uncps.
 
-  Definition cons_to_nth_cps {n} i (x:Z) (t:(list Z)^n)
-             {T} (f:(list Z)^n->T) :=
-    @on_tuple_cps _ _ nil (update_nth_cps i (cons x)) n n t _ f.
+    Definition nils n : (list Z)^n :=
+      Tuple.repeat nil n.
 
-  Definition nils n : (list Z)^n :=
-    from_list n (repeat nil n) (repeat_length _ _).
+    Lemma map_sum_nils n : map sum (nils n) = B.Positional.zeros n.
+    Proof.
+      cbv [nils B.Positional.zeros]; induction n; [reflexivity|].
+      change (repeat nil (S n)) with (@nil Z :: repeat nil n).
+      rewrite map_repeat, sum_nil. reflexivity.
+    Qed.
 
-  Definition from_associational_cps n (p:list B.limb)
-             {T} (f:(list Z)^n -> T) :=
-    fold_right_cps
-      (fun t st =>
-         B.Positional.place_cps weight t (pred n)
-                   (fun p=> cons_to_nth_cps (fst p) (snd p) st id))
-      (nils n) p f.
-  
-  Definition mul_cps {n m} (p q : Z^n) {T} (f : (list Z)^m->T) :=
-    B.Positional.to_associational_cps weight p
-      (fun P => B.Positional.to_associational_cps weight q
-      (fun Q => B.Associational.mul_cps P Q
-       (fun PQ => from_associational_cps m PQ f))). 
+    Lemma eval_nils n : eval (nils n) = 0.
+    Proof. cbv [eval]. rewrite map_sum_nils, B.Positional.eval_zeros. reflexivity. Qed.
 
-End Saturated.
+    Definition from_associational_cps n (p:list B.limb)
+               {T} (f:(list Z)^n -> T) :=
+      fold_right_cps
+        (fun t st =>
+           B.Positional.place_cps weight t (pred n)
+             (fun p=> cons_to_nth_cps (fst p) (snd p) st id))
+        (nils n) p f.
+    
+    Definition mul_cps {n m} (p q : Z^n) {T} (f : (list Z)^m->T) :=
+      B.Positional.to_associational_cps weight p
+        (fun P => B.Positional.to_associational_cps weight q
+        (fun Q => B.Associational.mul_cps P Q
+        (fun PQ => from_associational_cps m PQ f))).
+    
+    Definition add_cps {n} (p q : Z^n) {T} (f : (list Z)^n->T) :=
+      B.Positional.to_associational_cps weight p
+        (fun P => B.Positional.to_associational_cps weight q
+        (fun Q => from_associational_cps n (P++Q) f)).
+
+  End Saturated.
+End Sorted.
 
 (*
 (* Just some pretty-printing *)
@@ -187,11 +218,17 @@ Local Notation "snd~ a" := (let (_,y) := a in y) (at level 40, only printing).
 Definition base10 i := Eval compute in 10^(Z.of_nat i).
 Eval cbv -[runtime_add runtime_mul Let_In] in
     (fun adc a0 a1 a2 b0 b1 b2 =>
-       mul_cps (weight := base10) (n:=3) (a2,a1,a0) (b2,b1,b0) (fun ab => compact (n:=5) (add_get_carry:=adc) (weight:=base10) ab)).
+       Sorted.mul_cps (weight := base10) (n:=3) (a2,a1,a0) (b2,b1,b0) (fun ab => Sorted.compact (n:=5) (add_get_carry:=adc) (weight:=base10) ab)).
 
-(* More complex example : base 56, 8 limbs *)
+(* More complex example : base 2^56, 8 limbs *)
 Definition base2pow56 i := Eval compute in 2^(56*Z.of_nat i).
-Eval cbv -[runtime_add runtime_mul Let_In] in
+Time Eval cbv -[runtime_add runtime_mul Let_In] in
     (fun adc a0 a1 a2 a3 a4 a5 a6 a7 b0 b1 b2 b3 b4 b5 b6 b7 =>
-       mul_cps (weight := base10) (n:=8) (a7,a6,a5,a4,a3,a2,a1,a0) (b7,b6,b5,b4,b3,b2,b1,b0) (fun ab => compact (n:=15) (add_get_carry:=adc) (weight:=base10) ab)).
+       Sorted.mul_cps (weight := base2pow56) (n:=8) (a7,a6,a5,a4,a3,a2,a1,a0) (b7,b6,b5,b4,b3,b2,b1,b0) (fun ab => Sorted.compact (n:=15) (add_get_carry:=adc) (weight:=base2pow56) ab)). (* Finished transaction in 151.392 secs *) 
+
+(* Mixed-radix example : base 2^25.5, 10 limbs *)
+Definition base2pow25p5 i := Eval compute in 2^(25*Z.of_nat i + ((Z.of_nat i + 1) / 2)).
+Time Eval cbv -[runtime_add runtime_mul Let_In] in
+    (fun adc a0 a1 a2 a3 a4 a5 a6 a7 a8 a9 b0 b1 b2 b3 b4 b5 b6 b7 b8 b9 =>
+       Sorted.mul_cps (weight := base2pow25p5) (n:=10) (a9,a8,a7,a6,a5,a4,a3,a2,a1,a0) (b9,b8,b7,b6,b5,b4,b3,b2,b1,b0) (fun ab => Sorted.compact (n:=19) (add_get_carry:=adc) (weight:=base2pow25p5) ab)). (* Finished transaction in 97.341 secs *)
 *)
